Model and other methods

src/Knapsack/Implementation/PQ.dfy
@@ -1,26 +1,22 @@
-//include "Implementation/Solution.dfy"
+//include "PQData.dfy"
 
-abstract module Q {
+abstract module PQ {
   class Solution {
     var priority : real
 
-    ghost predicate Compare(other : Solution)
+    predicate Compare(other : Solution)
       reads this, other
-    {
-      this.priority < other.priority
-    }
+
   }
 
-  /*
-   The following priority queue is implemented with a williams heap (binary heap)
-  */
+  /* The following priority queue is implemented with a williams heap (binary heap) */
   class PriorityQueue {
     var arr : array<Solution>
     var count : int  // current number of elements, if count == arr.Length, array must grow
 
 
     constructor PriorityQueue(size: int)
-      //ensures this.Valid()
+      //ensures Valid()
     {
       this.arr := new Solution[0];
       this.count := 0;
@@ -30,7 +26,7 @@ abstract module Q {
     /* Predicates */
 
     /* Predicate: true if the segment [x, y) of the array satisfies the heap property*/
-    predicate isHeap(x : int, y : int)
+    predicate IsHeap(x : int, y : int)
       reads this, this.arr, set i | 0 <= i < this.arr.Length :: arr[i]
     {
       && 0 <= x <= y <= arr.Length
@@ -41,7 +37,7 @@ abstract module Q {
     predicate Valid()
       reads this, this.arr, set i | 0 <= i < this.arr.Length :: arr[i]
     {
-      this.isHeap(0, this.count)
+      IsHeap(0, this.count)
     }
 
 
@@ -53,8 +49,42 @@ abstract module Q {
     }
 
 
+    /* Predicate: true if m is the node with the minimum priority in the heap, i.e., no other node in the heap has a lower priority. */
+    predicate IsMin(m : Solution)
+      reads this, this.arr, m, set i | i in Model()
+      requires this.arr.Length == this.count
+      requires !IsEmpty()
+    {
+      && m in Model() // m belongs to the model
+      && forall i : Solution | i in Model() :: m.priority <= i.priority // the priority of m is not greater than any element of the set
+    }
+
+
+    /* Functions */
+
+    /* Function: returns the model of the heap */
+    function Model() : set<Solution>
+      reads this, this.arr
+      requires !IsEmpty()
+      requires this.arr.Length == this.count
+      ensures forall i : Solution | i in Model() :: (exists j | 0 <= j < this.count :: i == this.arr[j])
+    {
+      set j | 0 <= j < this.count :: this.arr[j]
+    }
+
 
     /* Methods */
+
+    /* Method: returns the element with the minimum priority in the heap */
+    // method Min() returns (node : Solution)
+    //   requires !IsEmpty()
+    //   requires Valid()
+    //   requires this.arr.Length == this.count
+    //   ensures IsMin(node)
+    // {
+    //   return this.arr[0];
+    // }
+
 
     /* Method: returns the current number of elements in the heap */
     method Size() returns (c : int)
@@ -63,22 +93,34 @@ abstract module Q {
     }
 
 
-    /* Method: returns the element with the minimum priority in the heap */
-    method Min() returns (m : Solution)
-      requires 0 < this.count <= this.arr.Length <= this.arr.Length
-      requires this.Valid()
+    /* Method: returns the model of the heap */
+    method Model2() returns (s: set<Solution>)
+      requires !IsEmpty()
+      requires this.arr.Length == this.count
+      ensures forall i : Solution | i in s :: (exists j | 0 <= j < this.count :: i == this.arr[j])
     {
-      return this.arr[0];
+      var aux: set<Solution> := {};
+      var j := 0;
+      while j < this.count
+        decreases this.count - j
+        invariant 0 <= j <= this.count
+        invariant forall i : Solution | i in aux :: (exists k | 0 <= k < j :: i == this.arr[k])
+      {
+        aux := aux + {this.arr[j]};
+        j := j + 1;
+      }
+      s := aux;
     }
 
 
     /* Method: inserts an element to the heap */
     method Insert(node : Solution)
       modifies this, this.arr
-      requires this.Valid()
-      //ensures this.Valid()
+      requires Valid()
+      ensures Valid()
+      ensures !IsEmpty()
+      //ensures IsMin(this.arr[0])
     {
-
       if (this.IsEmpty()) {
         var aux: array<Solution> := new Solution[1][node];
         this.arr := aux;
@@ -91,14 +133,15 @@ abstract module Q {
         this.arr[this.count] := node;
       }
       this.count := this.count + 1;
-      this.Float();      
+      this.Float();
     }
 
 
     /* Method: duplicates space of the heap */
-    method Grow()        
+    method Grow()
       modifies this, this.arr
-      requires 0 < this.count == this.arr.Length
+      requires !IsEmpty()
+      requires this.count == this.arr.Length
       ensures this.count == old(this.count) // the number of elements does not change in this method. The Method Insert increases it
       ensures this.arr.Length > old(this.arr.Length) // the length of the array increases
       ensures fresh(this.arr) // is new in memory
@@ -120,9 +163,7 @@ abstract module Q {
         i := i + 1;
       }
       assert aux[0..this.count] == this.arr[0..this.count] == old(this.arr[0..this.count]);
-      //assert Seq.Rev(aux[0..size]) == Seq.Rev(list[0..size]) == Seq.Rev(old(list[0..size]));
       this.arr := aux;
-      //assert Model() == Seq.Rev(aux[0..size]);
     }
 
 
@@ -131,7 +172,7 @@ abstract module Q {
       modifies this.arr
       requires 0 < this.count <= this.arr.Length
       requires forall i | 0 < i < this.count - 1 :: this.arr[(i-1)/2].priority <= this.arr[i].priority
-      ensures this.Valid()
+      ensures Valid()
     // {
     //     var j := this.count - 1;
     //     while j > 0 && this.arr[(j-1)/2].priority > this.arr[j].priority
@@ -148,9 +189,10 @@ abstract module Q {
     /* Method: deletes the element with the minimum priority of the heap */
     method DeleteMin()
       modifies this, this.arr
-      requires this.Valid()
-      requires 0 < this.count
-      //ensures this.Valid()
+      requires Valid()
+      requires !IsEmpty()
+      //ensures Model() == old(Model()) - {Min()}
+      //ensures Valid()
     {
       this.arr[0] := this.arr[this.count - 1];
       this.count := this.count - 1;
@@ -163,7 +205,7 @@ abstract module Q {
       modifies this.arr
       requires 0 <= s <= l == this.count <= arr.Length
       requires forall i | 0 < i < this.count && (i-1)/2 != s :: this.arr[(i-1)/2].priority <= this.arr[i].priority
-      ensures this.Valid()
+      ensures Valid()
 
 
   }
