src/Knapsack/Implementation/KnapsackPQ.dfy
@@ -1,0 +1,16 @@
+include "PQ.dfy"
+
+module KnapsackPQ refines PQ {
+  class Payload {
+    var s : Solution
+
+    constructor (s: Solution)
+      ensures this.s == s
+    {
+      this.s := s;
+    }
+  }
+
+  // Aquí no implementamos Compare, sigue abstracto.
+  // La idea es que el usuario lo tenga que implementar en su Solution.
+}
