src/Knapsack/Specification/PQData.dfy
@@ -1,0 +1,10 @@
+include "Solution.dfy"
+
+class PQData {
+    var s : set<Solution>
+
+    constructor PQData()
+    {
+      this.s := {};
+    }
+}
